Mostly complete concurrent queue example.

progs/verif_queue_ex.v
@@ -43,7 +43,7 @@ Notation f_lock_inv lsh gsh gsh1 gsh2 p' p lock t locksp lockt resultsp :=
   (EX p1 : val, EX p2 : val, EX p3 : val, EX i1 : int, EX i2 : int, EX i3 : int,
      data_at gsh (tptr tqueue_t) p p' *
      lqueue lsh tint (tc_val tint) p lock gsh1 gsh2
-       [@QRem tint p1 (Vint i1); @QRem tint p2 (Vint i2); @QRem tint p3 (Vint i3)] *
+       [QRem p1 (Vint i1); QRem p2 (Vint i2); QRem p3 (Vint i3)] *
      data_at gsh (tarray (tptr tlock) 3) (upd_Znth t (repeat Vundef 3) lockt) locksp *
      field_at Ews (tarray (tarray tint 3) 3) [ArraySubsc t] [Vint i1; Vint i2; Vint i3] resultsp).
 
@@ -82,11 +82,11 @@ Proof.
   intros; unfold f_lock_pred.
   apply selflock_precise.
   apply derives_precise' with (Q := data_at gsh (tptr tqueue_t) p p' *
-    (EX h : hist tint, lqueue lsh tint (tc_val tint) p lock gsh1 gsh2 h) *
+    (EX h : hist (reptype tint), lqueue lsh tint (tc_val tint) p lock gsh1 gsh2 h) *
     data_at gsh (tarray (tptr tlock) 3) (upd_Znth t (repeat Vundef 3) lockt) locksp *
     field_at_ Ews (tarray (tarray tint 3) 3) [ArraySubsc t] resultsp).
   - Intros p1 p2 p3 i1 i2 i3; cancel.
-    Exists [@QRem tint p1 (Vint i1); @QRem tint p2 (Vint i2); @QRem tint p3 (Vint i3)]; auto.
+    Exists [QRem p1 (Vint i1); QRem p2 (Vint i2); QRem p3 (Vint i3)]; auto.
   - repeat apply precise_sepcon; auto.
 Qed.
 
@@ -130,13 +130,13 @@ Proof.
          data_at gsh (tarray (tptr tlock) 3) (upd_Znth t [Vundef; Vundef; Vundef] lockt) locksp;
          lock_inv tsh lockt (f_lock_pred lsh gsh tsh gsh1 gsh2 p' p lock t locksp lockt resultsp);
          EX vals : _, !!(Zlength vals = i) &&
-           (lqueue lsh tint (tc_val tint) p lock gsh1 gsh2 (map (fun x => @QRem tint (fst x) (Vint (snd x))) vals) *
+           (lqueue lsh tint (tc_val tint) p lock gsh1 gsh2 (map (fun x => QRem (fst x) (Vint (snd x))) vals) *
             field_at Ews (tarray (tarray tint 3) 3) [ArraySubsc t]
               (map (fun x => Vint (snd x)) vals ++ repeat Vundef (Z.to_nat (3 - i))) resultsp))).
   { Exists ([] : list (val * int)); repeat entailer!. }
   { Intros vals.
-    forward_call (lsh, existT (fun t => ((reptype t -> Prop) * hist t)%type) tint (tc_val tint,
-      map (fun x => @QRem tint (fst x) (Vint (snd x))) vals), p, lock, gsh1, gsh2).
+    forward_call (lsh, existT (fun t => ((reptype t -> Prop) * hist (reptype t))%type) tint (tc_val tint,
+      map (fun x => QRem (fst x) (Vint (snd x))) vals), p, lock, gsh1, gsh2).
     Intros x; destruct x as (p1 & v1).
     simpl; forward.
     replace_SEP 1 (memory_block Tsh (sizeof tint) p1).
@@ -200,21 +200,6 @@ Qed.*)
 
 Opaque upto.
 
-(* This should probably be proved higher up, and used regularly. *)
-Lemma data_at__eq : forall sh t p, data_at_ sh t p = data_at sh t (default_val t) p.
-Proof.
-  intros; unfold data_at_, data_at, field_at_; auto.
-Qed.
-
-Lemma combine_snd : forall {A B} (l : list A) (l' : list B), length l = length l' ->
-  map snd (combine l l') = l'.
-Proof.
-  induction l; destruct l'; try discriminate; auto; intros.
-  inv H; simpl; rewrite IHl; auto.
-Qed.
-
-Set Default Timeout 60.
-
 Lemma main_loop1 : forall {Espec : OracleKind} (q0 locks results lvar0 : val) q lock
   lshs1 (Hlenl1 : Zlength lshs1 = 3)
   (Hlshs1 : forall i : Z, 0 <= i < 3 -> let '(a, b) := Znth i lshs1 (Tsh, Tsh) in
@@ -233,7 +218,7 @@ semax (initialized_list [_i; _i__1; _t'1] (func_tycontext f_main Vprog Gprog))
    gvar _q0 q0)
    SEP (lqueue (fst (Znth (3 - i) lshs1 (Tsh, Tsh))) tint (is_int I32 Signed) q lock sh1 sh2 [];
    data_at_ Ews (tarray (tarray tint 3) (3 - i))
-     (offset_val (nested_field_offset (tarray tint 3) [ArraySubsc i]) results);
+     (offset_val (nested_field_offset (tarray (tarray tint 3) 3) [ArraySubsc i]) results);
    field_at (fst (Znth (3 - i) gshs1 (Ews, Ews))) (tptr tqueue_t) [] q q0;
    data_at (fst (Znth (3 - i) gshs1 (Ews, Ews))) (tarray (tptr (Tstruct _lock_t noattr)) 3) flocks locks;
    fold_right sepcon emp
@@ -261,7 +246,7 @@ semax (initialized_list [_i; _i__1; _t'1] (func_tycontext f_main Vprog Gprog))
       gvar _q0 q0)
       SEP (lqueue (fst (Znth (3 - (i + 1)) lshs1 (Tsh, Tsh))) tint (is_int I32 Signed) q lock sh1 sh2 [];
       data_at_ Ews (tarray (tarray tint 3) (3 - (i + 1)))
-        (offset_val (nested_field_offset (tarray tint 3) [ArraySubsc (i + 1)]) results);
+        (offset_val (nested_field_offset (tarray (tarray tint 3) 3) [ArraySubsc (i + 1)]) results);
       field_at (fst (Znth (3 - (i + 1)) gshs1 (Ews, Ews))) (tptr tqueue_t) [] q q0;
       data_at (fst (Znth (3 - (i + 1)) gshs1 (Ews, Ews))) (tarray (tptr (Tstruct _lock_t noattr)) 3) flocks locks;
       fold_right sepcon emp
@@ -282,6 +267,20 @@ Proof.
   match goal with |-context[mk_funspec ?a ?b (rmaps.ConstType ?c) (fun _ => ?d) (fun _ => ?e) _ _] =>
     change (mk_funspec _ _ _ _ _ _ _) with (NDmk_funspec a b c d e) end.
   apply extract_exists_pre; intros f_.
+  specialize (Hgshs1 (2 - i)); exploit Hgshs1; [abstract omega|].
+  destruct (Znth (2 - i) gshs1 (Ews, Ews)) eqn: Hg1.
+  replace (2 - i + 1) with (3 - i) by abstract omega.
+  intros (? & ? & Hglsh); rewrite <- (data_at_share_join _ _ _ _ _ _ Hglsh),
+    <- (field_at_share_join _ _ _ _ _ _ _ Hglsh); auto.
+  specialize (Hlshs1 (2 - i)); exploit Hlshs1; [omega|].
+  destruct (Znth (2 - i) lshs1 (Tsh, Tsh)) eqn: Hl1.
+  replace (2 - i + 1) with (3 - i) by abstract omega.
+  intros (? & ? & Hllsh); replace_SEP 3 (lqueue s tint (tc_val tint) q lock sh1 sh2 [] *
+    lqueue s0 tint (tc_val tint) q lock sh1 sh2 []).
+  { go_lowerx.
+    rewrite sepcon_emp; apply lqueue_share_join_nil; auto. }
+  assert (length (upto 3) = length flocks).
+  { rewrite upto_length; rewrite Zlength_correct in *; abstract Omega0. }
   forward_spawn (share * share * share * share * share * val * val * val * Z * val * val * val)%type
     (f_, t, (snd (Znth (2 - i) lshs1 (Tsh, Tsh)), snd (Znth (2 - i) gshs1 (Ews, Ews)), sh2, sh1, sh2, q0, q,
              lock, i, locks, Znth i flocks Vundef, results),
@@ -295,38 +294,27 @@ Proof.
         data_at gsh (tarray (tptr tlock) 3) (upd_Znth t (repeat Vundef 3) lockt) locksp;
         field_at_ Ews (tarray (tarray tint 3) 3) [ArraySubsc t] resultsp;
         lock_inv tsh lockt (f_lock_pred lsh gsh tsh gsh1 gsh2 p' p lock t locksp lockt resultsp)]).
-  { Timeout 100 entailer!.
+  { unfold spawn_pre; go_lower.
+    entailer!.
     { rewrite sem_cast_neutral_ptr; rewrite sem_cast_neutral_ptr; auto.
-      split; auto; split; [apply Forall_Znth; auto; omega|].
-      specialize (Hlshs1 (2 - i)); exploit Hlshs1; [omega|].
-      destruct (Znth (2 - i) lshs1 (Tsh, Tsh)).
-      specialize (Hgshs1 (2 - i)); exploit Hgshs1; [omega|].
-      destruct (Znth (2 - i) gshs1 (Ews, Ews)); tauto. }
+      rewrite Hg1, Hl1; repeat split; auto.
+      apply Forall_Znth; auto; omega. }
     Exists _arg (fun x : (share * share * share * share * share * val * val * val * Z * val * val * val) =>
       let '(lsh, gsh, tsh, gsh1, gsh2, p', p, lock, t, locksp, lockt, resultsp) := x in
       [(_q0, p'); (_thread_locks, locksp); (_results, resultsp)]).
     rewrite !sepcon_assoc; apply sepcon_derives.
     { apply derives_refl'.
-      f_equal; f_equal; extensionality; destruct x as (?, x); repeat destruct x as (x, ?); simpl; try reflexivity.
+      f_equal; f_equal; extensionality; destruct x as (?, x); repeat destruct x as (x, ?); simpl.
       rewrite !sepcon_emp; reflexivity. }
-      specialize (Hgshs1 (2 - i)); exploit Hgshs1; [omega|].
-      destruct (Znth (2 - i) gshs1 (Ews, Ews)) eqn: Hg1.
-      replace (2 - i + 1) with (3 - i) by omega.
-      intros (? & ? & Hglsh); rewrite <- (data_at_share_join _ _ _ _ _ _ Hglsh),
-        <- (field_at_share_join _ _ _ _ _ _ _ Hglsh); auto.
-    specialize (Hlshs1 (2 - i)); exploit Hlshs1; [omega|].
-    destruct (Znth (2 - i) lshs1 (Tsh, Tsh)) eqn: Hl1.
-    replace (2 - i + 1) with (3 - i) by omega.
-    intros (? & ? & Hllsh); rewrite <- (lqueue_share_join tint _ s s0 (fst (Znth (3 - i) lshs1 (Tsh, Tsh))))
-      with (h1 := [])(h2 := []); auto.
     erewrite sublist_split with (lo := i), <- Znth_cons_sublist;
       try rewrite Zlength_combine, Zlength_upto, Z.min_l; simpl; try omega.
-    instantiate (1 := (0, Vundef)).
-    rewrite <- Znth_map', combine_snd; [|rewrite upto_length; rewrite Zlength_correct in *; Omega0].
+    instantiate (1 := (3, Vundef)).
+    rewrite <- Znth_map', combine_snd; auto.
     rewrite <- (lock_inv_share_join sh1 sh2 Tsh); auto.
     unfold tarray at 1; erewrite data_at__eq, split2_data_at_Tarray with (n1 := 1); try apply eq_JMeq;
       try reflexivity; [| omega | rewrite sublist_same; auto].
-    Timeout 100 cancel.
+    rewrite Hg1, Hl1; simpl.
+    cancel.
     rewrite (sepcon_comm _ (data_at t1 _ _ _)); rewrite !sepcon_assoc; apply sepcon_derives.
     { rewrite lock_struct_array; apply stronger_array_ext.
       { unfold unfold_reptype; simpl.
@@ -334,406 +322,206 @@ Proof.
       intros; unfold unfold_reptype, default_val; simpl.
       destruct (eq_dec i0 i).
       - subst; rewrite upd_Znth_same; [apply stronger_refl | Omega0].
-      - rewrite upd_Znth_diff; auto; try Omega0.
+      - rewrite upd_Znth_diff; auto.
         rewrite Znth_repeat with (x := Vundef)(n0 := 3%nat); apply stronger_default_val. }
     rewrite <- !sepcon_assoc, (sepcon_comm (lqueue _ _ _ _ _ _ _ _)), !sepcon_assoc; apply sepcon_derives.
-    { unfold field_at_, data_at, field_at, at_offset; entailer!.
+    { eapply derives_trans; [|unfold field_at_; apply field_at_stronger, stronger_default_val].
+      unfold data_at, field_at, at_offset; entailer!.
       { eapply field_compatible_cons_Tarray; try eassumption; reflexivity. }
       rewrite data_at_rec_eq; simpl.
-    unfold f_lock.
-    Search Znth map.
-    specialize (Hgshs1 (2 - i)); exploit Hgshs1; [abstract omega|].
-    destruct (Znth (2 - i) gshs1 (Ews, Ews)) eqn: Hg1.
-    replace (2 - i + 1) with (3 - i) by abstract omega.
-    intros (? & ? & Hglsh); rewrite <- (data_at_share_join _ _ _ _ _ _ Hglsh); auto.
-    specialize (Hlshs1 (2 - i)); exploit Hlshs1; [abstract omega|].
-    destruct (Znth (2 - i) lshs1 (Tsh, Tsh)) eqn: Hl1.
-    replace (2 - i + 1) with (3 - i) by abstract omega.
-    intros (? & ? & Hllsh); rewrite <- (lqueue_share_join s s0 (fst (Znth (3 - i) lshs1 (Tsh, Tsh)))); auto.
-    unfold lqueue; simpl; rewrite Z.sub_add_distr, <- app_assoc; simpl.
-    repeat rewrite Hg1; repeat rewrite Hl1; simpl.
-    repeat rewrite sepcon_andp_prop'; apply andp_right; [apply prop_right; auto | cancel].
-    rewrite Z2Nat.inj_add, upto_app, combine_app; try abstract omega.
-    simpl; repeat rewrite map_app; simpl.
-    rewrite Z2Nat.id, Z.add_0_r, Hg1, Hl1; simpl; [|abstract omega].
-    rewrite sem_cast_neutral_ptr; auto.
-    rewrite sepcon_app; simpl; unfold fold_right at 2; cancel.
-    { rewrite upto_length; rewrite Zlength_correct in *; Omega0. } }
+      unfold array_pred, aggregate_pred.array_pred; simpl.
+      unfold at_offset.
+      rewrite offset_offset_val, Z.add_0_l, Z.add_0_r; entailer!. }
+    rewrite <- !sepcon_assoc, (sepcon_comm _ (lock_inv sh2 _ _)), !sepcon_assoc; apply sepcon_derives.
+    { apply derives_refl'; unfold f_lock; simpl; f_equal.
+      rewrite <- Znth_map' with (f := fst), combine_fst; [|assumption].
+      simpl; rewrite Znth_upto with (m := 3%nat); [|simpl; omega].
+      rewrite Hl1, Hg1; simpl.
+      rewrite <- Znth_map', combine_snd; [reflexivity | assumption]. }
+    cancel.
+    { unfold default_val; simpl.
+      rewrite Zlength_list_repeat; auto; abstract omega. } }
   entailer!.
-  replace (3 - (Zlength flocks + 1)) with (2 - Zlength flocks) by abstract omega.
-  Exists (flocks ++ [l]); rewrite Zlength_app, Zlength_cons, Zlength_nil; entailer!.
-Qed.*)
-Admitted.*)
-
-(*Lemma main_loop2 : forall {Espec : OracleKind} (q0 lvar0 : val) gsh1 gsh2 (Hgsh1 : readable_share gsh1) (Hgsh2 : readable_share gsh2)
-  (Hgsh : sepalg.join gsh1 gsh2 Ews) g1 g2 g3 (ghosts := [g1; g2; g3]) p lock lshs1 (Hlenl1 : Zlength lshs1 = 3)
-  (Hlshs1 : forall i : Z, 0 <= i < 3 -> let '(a, b) := Znth i lshs1 (Tsh, Tsh) in
-          readable_share a /\ readable_share b /\ sepalg.join a b (fst (Znth (i + 1) lshs1 (Tsh, Tsh))))
-  gshs1 (Hglen1 : Zlength gshs1 = 3)
-  (Hgshs1 : forall i : Z, 0 <= i < 3 -> let '(a, b) := Znth i gshs1 (Ews, Ews) in
-          readable_share a /\ readable_share b /\ sepalg.join a b (fst (Znth (i + 1) gshs1 (Ews, Ews))))
-  sh1 sh2 (Hsh1 : readable_share sh1) (Hsh2 : readable_share sh2) (Hsh : sepalg.join sh1 sh2 Tsh)
-  (f_lock := fun x : Z * val =>
-          Lock_inv sh1 (snd x)
-            (f_lock_pred (snd (Znth (2 - fst x) lshs1 (Tsh, Tsh))) (snd (Znth (2 - fst x) gshs1 (Ews, Ews))) sh2
-               q0 p lock (snd x) ghosts gsh2)) flocks (Hflocks : Zlength flocks = 3)
-  (lsh' := fst (Znth 0 lshs1 (Tsh, Tsh))) (gsh' := fst (Znth 0 gshs1 (Ews, Ews)))
-  lshs2 (Hlenl2 : Zlength lshs2 = 3)
-  (Hlshs2 : forall i : Z, 0 <= i < 3 -> let '(a, b) := Znth i lshs2 (lsh', lsh') in
-          readable_share a /\ readable_share b /\ sepalg.join a b (fst (Znth (i + 1) lshs2 (lsh', lsh'))))
-  gshs2 (Hglen2 : Zlength gshs2 = 3)
-  (Hgshs2 : forall i : Z, 0 <= i < 3 -> let '(a, b) := Znth i gshs2 (gsh', gsh') in
-          readable_share a /\ readable_share b /\ sepalg.join a b (fst (Znth (i + 1) gshs2 (gsh', gsh'))))
-  (g_lock := fun x : Z * val => Lock_inv sh1 (snd x)
-            (g_lock_pred (snd (Znth (2 - fst x) lshs2 (lsh', lsh'))) (snd (Znth (2 - fst x) gshs2 (gsh', gsh')))
-               sh2 q0 p lock (snd x) ghosts gsh1 gsh2 (Znth (fst x) ghosts Vundef))) i (Hi : 0 <= i < 3),
-semax (initialized_list [_i; _i__1; _t'1] (func_tycontext f_main Vprog Gprog))
-  (PROP (Zlength flocks = 3)
-   LOCAL (temp _i__1 (vint i); temp _t'1 p; lvar _thread_locks (tarray (tptr (Tstruct _lock_t noattr)) 6) lvar0;
-   gvar _q0 q0)
-   SEP (ghost_factory; data_at (fst (Znth (3 - i) gshs2 (gsh', gsh'))) (tptr tqueue_t) p q0;
-   lqueue (fst (Znth (3 - i) lshs2 (lsh', lsh'))) gsh2 p ghosts lock;
-   fold_right sepcon emp (skipn (Z.to_nat i) (map (ghost gsh1 tint (vint (-1))) ghosts));
-   fold_right sepcon emp (map Interp (map f_lock (combine (upto 3) flocks)));
-   EX glocks : list val,
-   !! (Zlength glocks = i) &&
-   (data_at Tsh (tarray (tptr (Tstruct _lock_t noattr)) 6) (flocks ++ glocks ++ repeat Vundef (Z.to_nat (3 - i)))
-      lvar0 * fold_right sepcon emp (map Interp (map g_lock (combine (upto (Z.to_nat i)) glocks))))))
-  (Ssequence
-     (Ssequence
-        (Scall (Some _t'3) (Evar _malloc (Tfunction (Ctypes.Tcons tuint Ctypes.Tnil) (tptr tvoid) cc_default))
-           [Esizeof (Tstruct _lock_t noattr) tuint])
-        (Sset _l__1 (Ecast (Etempvar _t'3 (tptr tvoid)) (tptr (Tstruct _lock_t noattr)))))
-     (Ssequence
-        (Sassign
-           (Ederef
-              (Ebinop Oadd (Evar _thread_locks (tarray (tptr (Tstruct _lock_t noattr)) 6))
-                 (Ebinop Oadd (Etempvar _i__1 tint) (Econst_int (Int.repr 3) tint) tint)
-                 (tptr (tptr (Tstruct _lock_t noattr)))) (tptr (Tstruct _lock_t noattr)))
-           (Etempvar _l__1 (tptr (Tstruct _lock_t noattr))))
-        (Ssequence
-           (Scall None (Evar _makelock (Tfunction (Ctypes.Tcons (tptr tvoid) Ctypes.Tnil) tvoid cc_default))
-              [Ecast (Etempvar _l__1 (tptr (Tstruct _lock_t noattr))) (tptr tvoid)])
-           (Scall None
-              (Evar _spawn
-                 (Tfunction
-                    (Ctypes.Tcons
-                       (tptr (Tfunction (Ctypes.Tcons (tptr tvoid) Ctypes.Tnil) (tptr tvoid) cc_default))
-                       (Ctypes.Tcons (tptr tvoid) Ctypes.Tnil)) tvoid cc_default))
-              [Ecast
-                 (Eaddrof (Evar _g (Tfunction (Ctypes.Tcons (tptr tvoid) Ctypes.Tnil) (tptr tvoid) cc_default))
-                    (tptr (Tfunction (Ctypes.Tcons (tptr tvoid) Ctypes.Tnil) (tptr tvoid) cc_default)))
-                 (tptr tvoid); Ecast (Etempvar _l__1 (tptr (Tstruct _lock_t noattr))) (tptr tvoid)]))))
-  (normal_ret_assert
-     (PROP (0 <= i + 1 <= 3; Zlength flocks = 3)
-      LOCAL (temp _i__1 (vint i); temp _t'1 p;
-      lvar _thread_locks (tarray (tptr (Tstruct _lock_t noattr)) 6) lvar0; gvar _q0 q0)
-      SEP (ghost_factory; data_at (fst (Znth (3 - (i + 1)) gshs2 (gsh', gsh'))) (tptr tqueue_t) p q0;
-      lqueue (fst (Znth (3 - (i + 1)) lshs2 (lsh', lsh'))) gsh2 p ghosts lock;
-      fold_right sepcon emp (skipn (Z.to_nat (i + 1)) (map (ghost gsh1 tint (vint (-1))) ghosts));
-      fold_right sepcon emp (map Interp (map f_lock (combine (upto 3) flocks)));
-      EX glocks : list val,
-      !! (Zlength glocks = i + 1) &&
-      (data_at Tsh (tarray (tptr (Tstruct _lock_t noattr)) 6)
-         (flocks ++ glocks ++ repeat Vundef (Z.to_nat (3 - (i + 1)))) lvar0 *
-       fold_right sepcon emp (map Interp (map g_lock (combine (upto (Z.to_nat (i + 1))) glocks))))))).
-Proof.
-  intros.
-  forward_call (sizeof tlock).
-    { simpl fold_right; cancel. }
-    { simpl; computable. }
-    Intros l glocks.
-    forward.
-    rewrite app_assoc, upd_Znth_app2; [|rewrite Zlength_app, Zlength_repeat; abstract omega].
-    rewrite Zlength_app; replace (i + 3 - (Zlength flocks + Zlength glocks)) with 0 by abstract omega.
-    rewrite upd_Znth0, sublist_repeat; try rewrite Zlength_repeat, Z2Nat.id; try abstract omega.
-    assert (isptr l) by (destruct l; try contradiction; simpl; auto).
-    forward_call (l, Tsh, g_lock_pred (snd (Znth (2 - i) lshs2 (lsh', lsh')))
-      (snd (Znth (2 - i) gshs2 (gsh', gsh'))) sh2 q0 p lock l ghosts gsh1 gsh2 (Znth i ghosts Vundef)).
-    { repeat rewrite sem_cast_neutral_ptr; auto; apply prop_right; auto. }
-    { repeat rewrite sepcon_assoc; apply sepcon_derives; [|cancel].
-      rewrite memory_block_data_at_; [simpl; cancel | apply malloc_field_compatible; auto; simpl; try computable].
-      exists 2; auto. }
-    get_global_function'' _g; Intros.
-    apply extract_exists_pre; intros g_.
-    match goal with |-context[func_ptr' ?P] => set (spec := P) end.
-    forward_call (g_, l, existT (fun ty => ty * (ty -> val -> Pred))%type
-      (share * share * share * Z * val * val * val * list val * nat * val * share * share)%type
-      ((snd (Znth (2 - i) lshs2 (lsh', lsh')), snd (Znth (2 - i) gshs2 (gsh', gsh')),
-       sh2, -1, q0, p, lock, ghosts, Z.to_nat i, Znth i ghosts Vundef, gsh1, gsh2),
-     fun (x : (share * share * share * Z * val * val * val * list val * nat * val * share * share)) (lockt : val) =>
-     let '(lsh, gsh, tsh, t, p', p, lock, ghosts, i, g, gsh1, gsh2) := x in
-     Pred_list [Pred_prop (readable_share lsh /\ readable_share gsh /\ readable_share tsh /\
-         Int.min_signed <= t <= Int.max_signed /\ sepalg.join gsh1 gsh2 Ews /\ nth_error ghosts i = Some g);
-       Data_at _ gsh (tptr tqueue_t) p p'; 
-       Field_at _ lsh tqueue_t [StructField _lock] lock p;
-       Lock_inv lsh lock (lock_pred gsh2 p ghosts);
-       Lock_inv tsh lockt (g_lock_pred lsh gsh tsh p' p lock lockt ghosts gsh1 gsh2 g);
-       Ghost gsh1 tint (vint t) g])).
-    { apply prop_right; destruct l; try contradiction; auto. }
-    { unfold fold_right at 1.
-      Exists _arg (fun x : share * share * share * Z * val * val * val * list val * nat * val * share * share =>
-        let '(_, _, _, _, p', _, _, _, _, _, _, _) := x in [(_q0, p')]).
-      repeat rewrite sepcon_assoc; apply sepcon_derives.
-      { apply derives_refl'.
-        subst spec; f_equal; f_equal.
-        extensionality.
-        destruct x as (?, (((((((((((?, ?), ?), ?), ?), ?), ?), ?), ?), ?), ?), ?)); simpl.
-        rewrite interp_ghost; f_equal; f_equal.
-        unfold SEPx, lqueue; simpl; normalize. }
-      subst Frame; instantiate (1 := [ghost_factory;
-        data_at (fst (Znth (2 - i) gshs2 (gsh', gsh'))) (tptr tqueue_t) p q0;
-        lqueue (fst (Znth (2 - i) lshs2 (lsh', lsh'))) gsh2 p ghosts lock;
-        fold_right sepcon emp (skipn (Z.to_nat (i + 1)) (map (ghost gsh1 tint (vint (-1))) ghosts));
-        fold_right sepcon emp (map Interp (map f_lock (combine (upto 3) flocks)));
-        data_at Tsh (tarray (tptr (Tstruct _lock_t noattr)) 6) (flocks ++ (glocks ++ [l]) ++ repeat Vundef (Z.to_nat (3 - (i + 1)))) lvar0;
-        fold_right sepcon emp (map Interp (map g_lock (combine (upto (Z.to_nat (i + 1))) (glocks ++ [l]))))]).
-      rewrite <- (lock_inv_share_join sh1 sh2 Tsh); auto.
-      exploit (Hgshs2 (2 - i)); [abstract omega|].
-      fold gsh'; destruct (Znth (2 - i) gshs2 (gsh', gsh')) eqn: Hg1.
-      replace (2 - i + 1) with (3 - i) by abstract omega.
-      intros (? & ? & Hglsh); rewrite <- (data_at_share_join _ _ _ _ _ _ Hglsh).
-      exploit (Hlshs2 (2 - i)); [abstract omega|].
-      fold lsh'; destruct (Znth (2 - i) lshs2 (lsh', lsh')) eqn: Hl1.
-      replace (2 - i + 1) with (3 - i) by abstract omega.
-      intros (? & ? & Hllsh); rewrite <- (lqueue_share_join s s0 (fst (Znth (3 - i) lshs2 (lsh', lsh'))));
-        auto.
-      unfold lqueue; simpl; rewrite Z.sub_add_distr, <- app_assoc; simpl.
-      repeat rewrite Hg1; repeat rewrite Hl1; rewrite <- app_assoc; simpl.
-      repeat rewrite sepcon_andp_prop'; apply andp_right; [apply prop_right | unfold fold_right; cancel].
-      { split; [|split; [|split; [|split; [|split]]]]; auto; try computable.
-        unfold Znth; destruct (zlt i 0); [abstract omega|].
-        subst ghosts; erewrite nth_error_nth; simpl; eauto; Omega0. }
-      rewrite Z2Nat.inj_add, upto_app, combine_app; try abstract omega.
-      simpl; repeat rewrite map_app; simpl.
-      rewrite Z.add_0_r, Z2Nat.id; simpl; [|abstract omega].
-      rewrite sepcon_app; simpl; unfold fold_right; cancel.
-      erewrite <- (firstn_skipn 1 (skipn (Z.to_nat i) _)), skipn_skipn,
-        <- firstn_1_skipn with (d := ghost gsh1 tint (vint (-1)) Vundef), sepcon_app; [|Omega0].
-      rewrite nth_Znth, Z2Nat.id; [simpl | abstract omega].
-      rewrite Hg1, Hl1, sem_cast_neutral_ptr; auto.
-      erewrite interp_ghost, <- Znth_map' with (f := ghost _ _ _); subst ghosts; simpl;
-        unfold fold_right; cancel.
-      { subst; rewrite Zlength_correct, Nat2Z.id, upto_length; auto. } }
-    go_lower; Exists (glocks ++ [l]); entailer!.
-    - rewrite Zlength_app, Zlength_cons, Zlength_nil; auto.
-    - replace (3 - (Zlength glocks + 1)) with (2 - Zlength glocks) by abstract omega; apply derives_refl.
+  replace (3 - (i + 1)) with (2 - i) by abstract omega; rewrite Hg1, Hl1; simpl; cancel.
+  erewrite sublist_split with (mid := i)(hi := i + 1), sublist_len_1, map_app, sepcon_app;
+    try rewrite Zlength_combine, Zlength_upto, Z.min_l; simpl; try omega.
+  instantiate (1 := (3, Vundef)).
+  rewrite <- Znth_map' with (f := snd), combine_snd; simpl; unfold fold_right; [cancel | auto].
+  replace (3 - i - 1) with (2 - i) by (clear; omega).
+  unfold field_address0.
+  destruct (field_compatible0_dec _ _ _).
+  simpl; rewrite offset_offset_val.
+  rewrite Z.mul_add_distr_l; simpl; cancel.
+  { rewrite data_at_isptr; Intros; contradiction. }
+  { exists 2; auto. }
 Qed.
 
-Opaque upto.
-
-Lemma main_loop3 : forall {Espec : OracleKind} (q0 lvar0 : val) gsh1 gsh2 (Hgsh1 : readable_share gsh1) (Hgsh2 : readable_share gsh2)
-  (Hgsh : sepalg.join gsh1 gsh2 Ews) g1 g2 g3 (ghosts := [g1; g2; g3]) p lock lshs1 (Hlenl1 : Zlength lshs1 = 3)
-  (Hlshs1 : forall i : Z, 0 <= i < 3 -> let '(a, b) := Znth i lshs1 (Tsh, Tsh) in
-          readable_share a /\ readable_share b /\ sepalg.join a b (fst (Znth (i + 1) lshs1 (Tsh, Tsh))))
-  gshs1 (Hglen1 : Zlength gshs1 = 3)
-  (Hgshs1 : forall i : Z, 0 <= i < 3 -> let '(a, b) := Znth i gshs1 (Ews, Ews) in
-          readable_share a /\ readable_share b /\ sepalg.join a b (fst (Znth (i + 1) gshs1 (Ews, Ews))))
+Lemma main_loop2 : forall {Espec : OracleKind} (q0 q lock locks results : val)
   sh1 sh2 (Hsh1 : readable_share sh1) (Hsh2 : readable_share sh2) (Hsh : sepalg.join sh1 sh2 Tsh)
+  gshs1 (Hglen1 : Zlength gshs1 = 3) 
+  (Hgshs1 : forall i : Z,
+         0 <= i < 3 ->
+         let
+         '(a, b) := Znth i gshs1 (Ews, Ews) in
+          readable_share a /\ readable_share b /\ sepalg.join a b (fst (Znth (i + 1) gshs1 (Ews, Ews))))
+  lshs1 (Hlenl1 : Zlength lshs1 = 3)
+  (Hlshs1 : forall i : Z,
+         0 <= i < 3 ->
+         let
+         '(a, b) := Znth i lshs1 (Tsh, Tsh) in
+          readable_share a /\ readable_share b /\ sepalg.join a b (fst (Znth (i + 1) lshs1 (Tsh, Tsh))))
   (f_lock := fun x : Z * val =>
-          Lock_inv sh1 (snd x)
-            (f_lock_pred (snd (Znth (2 - fst x) lshs1 (Tsh, Tsh))) (snd (Znth (2 - fst x) gshs1 (Ews, Ews))) sh2
-               q0 p lock (snd x) ghosts gsh2)) flocks (Hflocks : Zlength flocks = 3)
+          f_lock_pred (snd (Znth (2 - fst x) lshs1 (Tsh, Tsh))) (snd (Znth (2 - fst x) gshs1 (Ews, Ews))) sh2 sh1
+            sh2 q0 q lock (fst x) locks (snd x) results)
+  flocks (Hfl : Zlength flocks = 3) (Hflocks : Forall isptr flocks)
+  (Hresults : field_compatible (tarray (tarray tint 3) 3) [] results)
   (lsh' := fst (Znth 0 lshs1 (Tsh, Tsh))) (gsh' := fst (Znth 0 gshs1 (Ews, Ews)))
-  lshs2 (Hlenl2 : Zlength lshs2 = 3)
-  (Hlshs2 : forall i : Z, 0 <= i < 3 -> let '(a, b) := Znth i lshs2 (lsh', lsh') in
-          readable_share a /\ readable_share b /\ sepalg.join a b (fst (Znth (i + 1) lshs2 (lsh', lsh'))))
-  gshs2 (Hglen2 : Zlength gshs2 = 3)
-  (Hgshs2 : forall i : Z, 0 <= i < 3 -> let '(a, b) := Znth i gshs2 (gsh', gsh') in
-          readable_share a /\ readable_share b /\ sepalg.join a b (fst (Znth (i + 1) gshs2 (gsh', gsh'))))
-  (g_lock := fun x : Z * val => Lock_inv sh1 (snd x)
-            (g_lock_pred (snd (Znth (2 - fst x) lshs2 (lsh', lsh'))) (snd (Znth (2 - fst x) gshs2 (gsh', gsh')))
-               sh2 q0 p lock (snd x) ghosts gsh1 gsh2 (Znth (fst x) ghosts Vundef)))
-  glocks (Hglocks : Zlength glocks = 3) i (Hi : 0 <= i < 6),
-semax (initialized_list [_i; _i__1; _i__2; _t'1] (func_tycontext f_main Vprog Gprog))
-  (PROP (Forall isptr flocks; Forall isptr glocks)
-   LOCAL (temp _i__2 (vint i); temp _t'1 p; lvar _thread_locks (tarray (tptr (Tstruct _lock_t noattr)) 6) lvar0;
+  (Hgsh' : readable_share gsh') ptrs (Hptrs : Zlength ptrs = 9) i (Hi : 0 <= i < 3),
+semax (initialized_list [_i; _i__1; _q1; _i__2; _i__3; _t'1] (func_tycontext f_main Vprog Gprog))
+  (PROP ( )
+   LOCAL (temp _i__3 (vint i); temp _q1 q; temp _t'1 q; gvar _results results; gvar _thread_locks locks;
    gvar _q0 q0)
-   SEP (ghost_factory; data_at (fst (Znth 0 gshs2 (gsh', gsh'))) (tptr tqueue_t) p q0;
+   SEP (field_at gsh' (tptr tqueue_t) [] q q0;
    fold_right sepcon emp
-     (firstn (Z.to_nat i)
-        (map (fun sh : Share.t => data_at sh (tptr tqueue_t) p q0) (map snd (rev gshs1 ++ rev gshs2))));
-   lqueue (fst (Znth 0 lshs2 (lsh', lsh'))) gsh2 p ghosts lock;
+     (sublist 0 i (map (fun sh : Share.t => data_at sh (tptr tqueue_t) q q0) (map snd (rev gshs1))));
+   data_at gsh' (tarray (tptr (Tstruct _lock_t noattr)) 3) flocks locks;
    fold_right sepcon emp
-     (firstn (Z.to_nat i)
-        (map (fun sh : Share.t => lqueue sh gsh2 p ghosts lock) (map snd (rev lshs1 ++ rev lshs2))));
-   EX ns : list Z,
-   !! (Zlength ns = Zlength ghosts) &&
+     (sublist 0 i
+        (map (fun sh : Share.t => data_at_ sh (tarray (tptr (Tstruct _lock_t noattr)) 3) locks)
+           (map snd (rev gshs1))));
    fold_right sepcon emp
-     (firstn (Z.to_nat i - 3) (map (fun x : Z * val => ghost gsh1 tint (vint (fst x)) (snd x)) (combine ns ghosts)));
-   fold_right sepcon emp (skipn (Z.to_nat i) (map Interp (map f_lock (combine (upto 3) flocks))));
-   fold_right sepcon emp (skipn (Z.to_nat i - 3) (map Interp (map g_lock (combine (upto 3) glocks))));
-   data_at Tsh (tarray (tptr (Tstruct _lock_t noattr)) 6) (flocks ++ glocks) lvar0))
+     (sublist i 3 (map (fun x : Z * val => lock_inv sh1 (snd x) (f_lock x)) (combine (upto 3) flocks)));
+   fold_right sepcon emp (sublist i 3 (map (fun x : val => malloc_token Tsh (sizeof tlock) x) flocks));
+   lqueue lsh' tint (is_int I32 Signed) q lock sh1 sh2
+     (map (fun x : val * Z => QAdd (fst x) (vint (snd x))) (combine ptrs (upto (Z.to_nat 9))));
+   EX vals : list (list (val * int)),
+   !! (Zlength vals = i /\ Forall (fun l : list (val * int) => Zlength l = 3) vals) &&
+   (fold_right sepcon emp
+      (map
+         (fun x : Share.t * list (val * int) =>
+          let
+          '(sh, vals0) := x in
+           lqueue sh tint (is_int I32 Signed) q lock sh1 sh2
+             (map (fun x0 : val * int => let '(p, i0) := x0 in QRem p (Vint i0)) vals0))
+         (combine (sublist 0 i (map snd (rev lshs1))) vals)) *
+    fold_right sepcon emp
+      (map
+         (fun x : Z =>
+          field_at Ews (tarray (tarray tint 3) 3) [ArraySubsc x] (map Vint (map snd (Znth x vals []))) results)
+         (upto (Z.to_nat i))))))
   (Ssequence
-     (Sset _l__2
+     (Sset _l__1
         (Ederef
-           (Ebinop Oadd (Evar _thread_locks (tarray (tptr (Tstruct _lock_t noattr)) 6)) 
-              (Etempvar _i__2 tint) (tptr (tptr (Tstruct _lock_t noattr)))) (tptr (Tstruct _lock_t noattr))))
+           (Ebinop Oadd (Evar _thread_locks (tarray (tptr (Tstruct _lock_t noattr)) 3)) 
+              (Etempvar _i__3 tint) (tptr (tptr (Tstruct _lock_t noattr)))) (tptr (Tstruct _lock_t noattr))))
      (Ssequence
-        (Scall None (Evar _acquire (Tfunction (Ctypes.Tcons (tptr tvoid) Ctypes.Tnil) tvoid cc_default))
-           [Ecast (Etempvar _l__2 (tptr (Tstruct _lock_t noattr))) (tptr tvoid)])
+        (Scall None (Evar _acquire (Tfunction (Tcons (tptr tvoid) Tnil) tvoid cc_default))
+           [Etempvar _l__1 (tptr (Tstruct _lock_t noattr))])
         (Ssequence
-           (Scall None (Evar _freelock2 (Tfunction (Ctypes.Tcons (tptr tvoid) Ctypes.Tnil) tvoid cc_default))
-              [Ecast (Etempvar _l__2 (tptr (Tstruct _lock_t noattr))) (tptr tvoid)])
-           (Scall None (Evar _free (Tfunction (Ctypes.Tcons (tptr tvoid) Ctypes.Tnil) tvoid cc_default))
-              [Etempvar _l__2 (tptr (Tstruct _lock_t noattr))]))))
+           (Scall None (Evar _freelock2 (Tfunction (Tcons (tptr tvoid) Tnil) tvoid cc_default))
+              [Etempvar _l__1 (tptr (Tstruct _lock_t noattr))])
+           (Scall None (Evar _free (Tfunction (Tcons (tptr tvoid) Tnil) tvoid cc_default))
+              [Etempvar _l__1 (tptr (Tstruct _lock_t noattr))]))))
   (normal_ret_assert
-     (PROP (0 <= i + 1 <= 6; Forall isptr flocks; Forall isptr glocks)
-      LOCAL (temp _i__2 (vint i); temp _t'1 p; lvar _thread_locks (tarray (tptr (Tstruct _lock_t noattr)) 6) lvar0;
+     (PROP (0 <= i + 1 <= 3)
+      LOCAL (temp _i__3 (vint i); temp _q1 q; temp _t'1 q; gvar _results results; gvar _thread_locks locks;
       gvar _q0 q0)
-      SEP (ghost_factory; data_at (fst (Znth 0 gshs2 (gsh', gsh'))) (tptr tqueue_t) p q0;
+      SEP (field_at gsh' (tptr tqueue_t) [] q q0;
       fold_right sepcon emp
-        (firstn (Z.to_nat (i + 1))
-           (map (fun sh : Share.t => data_at sh (tptr tqueue_t) p q0) (map snd (rev gshs1 ++ rev gshs2))));
-      lqueue (fst (Znth 0 lshs2 (lsh', lsh'))) gsh2 p ghosts lock;
+        (sublist 0 (i + 1) (map (fun sh : Share.t => data_at sh (tptr tqueue_t) q q0) (map snd (rev gshs1))));
+      data_at gsh' (tarray (tptr (Tstruct _lock_t noattr)) 3) flocks locks;
       fold_right sepcon emp
-        (firstn (Z.to_nat (i + 1))
-           (map (fun sh : Share.t => lqueue sh gsh2 p ghosts lock) (map snd (rev lshs1 ++ rev lshs2))));
-      EX ns : list Z,
-      !! (Zlength ns = Zlength ghosts) &&
+        (sublist 0 (i + 1)
+           (map (fun sh : Share.t => data_at_ sh (tarray (tptr (Tstruct _lock_t noattr)) 3) locks)
+              (map snd (rev gshs1))));
       fold_right sepcon emp
-        (firstn (Z.to_nat (i + 1) - 3)
-           (map (fun x : Z * val => ghost gsh1 tint (vint (fst x)) (snd x)) (combine ns ghosts)));
-      fold_right sepcon emp (skipn (Z.to_nat (i + 1)) (map Interp (map f_lock (combine (upto 3) flocks))));
-      fold_right sepcon emp (skipn (Z.to_nat (i + 1) - 3) (map Interp (map g_lock (combine (upto 3) glocks))));
-      data_at Tsh (tarray (tptr (Tstruct _lock_t noattr)) 6) (flocks ++ glocks) lvar0))).
+        (sublist (i + 1) 3 (map (fun x : Z * val => lock_inv sh1 (snd x) (f_lock x)) (combine (upto 3) flocks)));
+      fold_right sepcon emp (sublist (i + 1) 3 (map (fun x : val => malloc_token Tsh (sizeof tlock) x) flocks));
+      lqueue lsh' tint (is_int I32 Signed) q lock sh1 sh2
+        (map (fun x : val * Z => QAdd (fst x) (vint (snd x))) (combine ptrs (upto (Z.to_nat 9))));
+      EX vals : list (list (val * int)),
+      !! (Zlength vals = i + 1 /\ Forall (fun l : list (val * int) => Zlength l = 3) vals) &&
+      (fold_right sepcon emp
+         (map
+            (fun x : Share.t * list (val * int) =>
+             let
+             '(sh, vals0) := x in
+              lqueue sh tint (is_int I32 Signed) q lock sh1 sh2
+                (map (fun x0 : val * int => let '(p, i0) := x0 in QRem p (Vint i0)) vals0))
+            (combine (sublist 0 (i + 1) (map snd (rev lshs1))) vals)) *
+       fold_right sepcon emp
+         (map
+            (fun x : Z =>
+             field_at Ews (tarray (tarray tint 3) 3) [ArraySubsc x] (map Vint (map snd (Znth x vals []))) results)
+            (upto (Z.to_nat (i + 1)))))))).
 Proof.
   intros.
-  Intro ns; Intros.
-    forward.
-    { go_lower.
-      repeat apply andp_right; apply prop_right; auto.
-      apply Forall_Znth.
-      - rewrite Zlength_app; abstract omega.
-      - rewrite Forall_app; split; eapply Forall_impl; try eassumption; auto. }
-    destruct (Z_lt_dec i 3).
-    - rewrite app_Znth1; [|abstract omega].
-      forward_call (Znth i flocks Vundef, sh1, f_lock_pred (snd (Znth (2 - i) lshs1 (Tsh, Tsh)))
-        (snd (Znth (2 - i) gshs1 (Ews, Ews))) sh2 q0 p lock (Znth i flocks Vundef) ghosts gsh2).
-      { apply prop_right; rewrite eval_cast_neutral_is_pointer_or_null;
-          rewrite eval_cast_neutral_is_pointer_or_null; auto. }
-      { assert (length flocks = 3)%nat by (rewrite Zlength_correct in *; Omega0).
-        erewrite skipn_cons, !Znth_map', Znth_combine; auto;
-          [|rewrite !map_length, combine_length, Min.min_l; rewrite upto_length; Omega0].
-        rewrite Z2Nat.id; [|omega].
-        rewrite Znth_upto with (m := 3%nat); [|Omega0].
-        rewrite <- (Nat.add_1_r (Z.to_nat i)).
-        instantiate (1 := Vundef); simpl; cancel. }
-      freeze [2; 3; 4; 5; 6; 7; 8; 9; 10] FR.
-      forward_call (Znth i flocks Vundef, Tsh, Later (f_lock_pred (snd (Znth (2 - i) lshs1 (Tsh, Tsh)))
-        (snd (Znth (2 - i) gshs1 (Ews, Ews))) sh2 q0 p lock (Znth i flocks Vundef) ghosts gsh2)).
-      { apply prop_right; rewrite eval_cast_neutral_is_pointer_or_null;
-          rewrite eval_cast_neutral_is_pointer_or_null; auto. }
-      { simpl.
-        rewrite selflock_eq at 2.
-        rewrite (sepcon_comm (FRZL FR)); repeat rewrite sepcon_assoc.
-        eapply derives_trans; [apply sepcon_derives; [apply lock_inv_later | apply derives_refl]|].
-        rewrite <- (lock_inv_share_join sh1 sh2 Tsh); auto; cancel. }
-      { split; auto; split; [apply later_positive, f_inv_positive | apply later_rec, selflock_rec]. }
-      forward_call (Znth i flocks Vundef, sizeof tlock).
-      { rewrite data_at__memory_block; simpl; entailer!. }
-      Exists [0; 0; 0].
-      go_lower.
-      apply andp_right; [apply prop_right; repeat split; auto; abstract omega|].
-      apply andp_right; [apply prop_right; repeat split; auto|].
-      thaw FR.
-      rewrite Z2Nat.inj_add; try abstract omega; simpl.
-      assert (Z.to_nat i < 3)%nat by Omega0.
-      replace (Z.to_nat i + 1 - 3)%nat with O by abstract omega;
-        replace (Z.to_nat i - 3)%nat with O by abstract omega.
-      erewrite <- !firstn_app, <- !firstn_1_skipn.
-      rewrite !nth_Znth, !sepcon_app; simpl.
-      rewrite Z2Nat.id; try abstract omega.
-      rewrite !Znth_map', !app_Znth1; try (rewrite Zlength_rev; abstract omega).
-      rewrite !Znth_rev; try abstract omega.
-      rewrite Hglen1, Hlenl1.
-      replace (3 - i - 1) with (2 - i) by abstract omega.
-      unfold fold_right, lqueue; simpl; cancel.
-      entailer!.
-      apply derives_refl.
-      { rewrite !map_length, app_length, !rev_length.
-        rewrite Zlength_correct in *; Omega0. }
-      { rewrite !map_length, app_length, !rev_length.
-        rewrite Zlength_correct in *; Omega0. }
-    - rewrite app_Znth2; [|abstract omega].
-      replace (Zlength flocks) with 3 by auto.
-      assert (3 <= Z.to_nat i < 6)%nat.
-      { split; try Omega0.
-        rewrite Nat2Z.inj_le, Z2Nat.id; simpl; abstract omega. }
-      forward_call (Znth (i - 3) glocks Vundef, sh1, g_lock_pred (snd (Znth (2 - (i - 3)) lshs2 (lsh', lsh')))
-        (snd (Znth (2 - (i - 3)) gshs2 (gsh', gsh'))) sh2 q0 p lock (Znth (i - 3) glocks Vundef)
-        ghosts gsh1 gsh2 (Znth (i - 3) ghosts Vundef)).
-      { apply prop_right; rewrite eval_cast_neutral_is_pointer_or_null;
-          rewrite eval_cast_neutral_is_pointer_or_null; auto. }
-      { assert (length glocks = 3)%nat by (rewrite Zlength_correct in *; Omega0).
-        assert (3 > Z.to_nat i - 3)%nat by omega.
-        setoid_rewrite skipn_cons at 2;
-          [|rewrite !map_length, combine_length, Min.min_l; rewrite upto_length; auto; omega].
-        rewrite !Znth_map', Znth_combine, !Nat2Z.inj_sub, Z2Nat.id; auto; try omega.
-        rewrite Znth_upto with (m := 3%nat); [|simpl; omega].
-        rewrite <- (Nat.add_1_r (_ - _)).
-        instantiate (1 := Vundef); simpl; cancel. }
-      freeze [2; 3; 4; 5; 6; 7; 8; 9; 10] FR.
-      forward_call (Znth (i - 3) glocks Vundef, Tsh, Later (g_lock_pred
-        (snd (Znth (2 - (i - 3)) lshs2 (lsh', lsh')))
-        (snd (Znth (2 - (i - 3)) gshs2 (gsh', gsh'))) sh2 q0 p lock (Znth (i - 3) glocks Vundef)
-        ghosts gsh1 gsh2 (Znth (i - 3) ghosts Vundef))).
-      { apply prop_right; rewrite eval_cast_neutral_is_pointer_or_null;
-          rewrite eval_cast_neutral_is_pointer_or_null; auto. }
-      { simpl.
-        rewrite selflock_eq at 2.
-        rewrite (sepcon_comm (FRZL FR)); repeat rewrite sepcon_assoc.
-        eapply derives_trans; [apply sepcon_derives; [apply lock_inv_later | apply derives_refl]|].
-        rewrite <- (lock_inv_share_join sh1 sh2 Tsh); auto; cancel. }
-      { split; auto; split; [apply later_positive, g_inv_positive | apply later_rec, selflock_rec]. }
-      Intro x.
-      forward_call (Znth (i - 3) glocks Vundef, sizeof tlock).
-      { rewrite data_at__memory_block; simpl; entailer!. }
-      go_lower.
-      Exists (upd_Znth (i - 3) ns x).
-      apply andp_right; [apply prop_right; repeat split; auto; abstract omega|].
-      apply andp_right; [apply prop_right; repeat split; auto|].
-      thaw FR.
-      rewrite Z2Nat.inj_add; try abstract omega; simpl.
-      assert (Z.to_nat i < length gshs1 + length gshs2)%nat.
-      { rewrite Zlength_correct in *; Omega0. }
-      assert (Z.to_nat i < length lshs1 + length lshs2)%nat.
-      { rewrite Zlength_correct in *; Omega0. }
-      replace (Z.to_nat i + 1 - 3)%nat with (Z.to_nat i - 3 + 1)%nat by abstract omega.
-      assert (Zlength ns = 3).
-      { subst ghosts; rewrite !Zlength_cons, Zlength_nil in *; abstract omega. }
-      assert (length (upd_Znth (i - 3) ns x) = 3%nat).
-      { apply Nat2Z.inj.
-        rewrite <- Zlength_correct, upd_Znth_Zlength; simpl; abstract omega. }
-      erewrite <- !firstn_app, <- !firstn_1_skipn; try rewrite !map_length; try rewrite app_length, !rev_length;
-        try abstract omega.
-      rewrite !nth_Znth, !sepcon_app; simpl.
-      rewrite !Znth_map', !app_Znth2; try (rewrite Zlength_rev; abstract omega).
-      rewrite Nat2Z.inj_sub, Z2Nat.id; try abstract omega.
-      rewrite !Znth_rev; rewrite !Zlength_rev; try abstract omega.
-      rewrite interp_ghost, Znth_combine; auto; simpl.
-      instantiate (1 := Vundef); instantiate (1 := x).
-      rewrite upd_Znth_same; [|abstract omega].
-      assert (length flocks = 3%nat) by (rewrite Zlength_correct in *; Omega0).
-      rewrite skipn_short;
-        [|rewrite !map_length, combine_length, Min.min_l; rewrite upto_length; abstract omega].
-      setoid_rewrite skipn_short at 2;
-        [|rewrite !map_length, combine_length, Min.min_l; rewrite upto_length; abstract omega].
-      replace (Z.to_nat i - 3 + 1)%nat with (S (Z.to_nat i - 3))%nat by abstract omega.
-      rewrite Hglen1, Hlenl1, Hglen2, Hlenl2.
-      replace (3 - (i - 3) - 1) with (2 - (i - 3)) by abstract omega.
-      unfold fold_right, lqueue; simpl; cancel; entailer!.
-      + rewrite upd_Znth_Zlength; auto; abstract omega.
-      + rewrite sepcon_comm; apply sepcon_derives; [apply derives_refl|].
-        apply derives_refl'; f_equal.
-        replace (Z.to_nat i - 3)%nat with (Z.to_nat (i - 3)) by Omega0.
-        rewrite combine_upd_Znth1 with (d := Vundef), <- upd_Znth_map; try abstract omega.
-        rewrite <- !sublist_firstn, !sublist_upd_Znth_l; auto; try abstract omega.
-        rewrite Zlength_map.
-        rewrite Zlength_combine, Z.min_l; abstract omega.
-      + rewrite upd_Znth_Zlength; auto; abstract omega.
-      + rewrite combine_length, Min.min_r; subst ghosts; simpl; abstract omega.
-Qed.*)
+  Intros vals.
+  forward.
+  { entailer!.
+    apply Forall_Znth; [omega|].
+    eapply Forall_impl; [|apply Hflocks]; auto. }
+  forward_call (Znth i flocks Vundef, sh1, f_lock (i, Znth i flocks Vundef)).
+  { assert (Zlength (map (fun x => lock_inv sh1 (snd x) (f_lock x)) (combine (upto 3) flocks)) = 3).
+    { rewrite Zlength_map, Zlength_combine, Zlength_upto, Z.min_l; simpl; omega. }
+    assert (length (upto 3) = length flocks) by (rewrite upto_length; rewrite Zlength_correct in *; Omega0).
+    erewrite sublist_split with (lo := i), <- Znth_cons_sublist; try omega.
+    rewrite Znth_map', <- Znth_map', combine_snd; auto.
+    instantiate (1 := (3, Vundef)); simpl.
+    rewrite Znth_combine, Znth_upto; simpl; auto; [cancel | omega]. }
+  forward_call (Znth i flocks Vundef, Tsh, sh2, |>f_lock_inv (snd (Znth (2 - i) lshs1 (Tsh, Tsh)))
+    (snd (Znth (2 - i) gshs1 (Ews, Ews))) sh1 sh2 q0 q lock i locks (Znth i flocks Vundef) results,
+    |>f_lock (i, Znth i flocks Vundef)).
+  { simpl; lock_props.
+    - apply later_positive; unfold f_lock; apply f_inv_positive.
+      exploit (Hgshs1 (2 - i)); [omega|].
+      simpl; destruct (Znth (2 - i) gshs1 (Ews, Ews)); intros (? & ? & ?); auto.
+    - unfold rec_inv, f_lock, f_lock_pred.
+      rewrite selflock_eq at 1.
+      rewrite later_sepcon; f_equal.
+      apply lock_inv_later_eq.
+    - unfold f_lock at 2; unfold f_lock_pred; rewrite selflock_eq.
+      erewrite <- (lock_inv_share_join _ _ Tsh); try apply Hsh; auto.
+      rewrite !sepcon_assoc; apply sepcon_derives; [apply lock_inv_later|].
+      unfold f_lock at 2; unfold f_lock_pred; simpl snd; cancel. }
+  forward_call (Znth i flocks Vundef, sizeof tlock).
+  { rewrite data_at__memory_block.
+    erewrite sublist_split with (lo := i), <- Znth_cons_sublist; try rewrite Zlength_map; try omega.
+    rewrite Znth_map'.
+    instantiate (1 := Vundef); simpl; Intros; cancel. }
+  Intros p1 p2 p3 i1 i2 i3.
+  Exists (vals ++ [[(p1, i1); (p2, i2); (p3, i3)]]); rewrite Zlength_app.
+  entailer!.
+  { rewrite Forall_app; split; auto. }
+  erewrite sublist_split with (mid := Zlength vals)(hi := Zlength vals + 1), sublist_len_1;
+    rewrite ?Zlength_map, ?Zlength_rev; try omega.
+  rewrite 2Znth_map', Znth_rev; [|omega].
+  rewrite Hglen1, sepcon_app; instantiate (1 := (Ews, Ews)).
+  erewrite sublist_split with (mid := Zlength vals)(hi := Zlength vals + 1), sublist_len_1;
+    rewrite ?Zlength_map, ?Zlength_rev; try omega.
+  rewrite 2Znth_map', Znth_rev; [|omega].
+  rewrite Hglen1, sepcon_app; instantiate (1 := (Ews, Ews)).
+  erewrite sublist_split with (mid := Zlength vals)(hi := Zlength vals + 1), sublist_len_1;
+    rewrite ?Zlength_map, ?Zlength_rev; try omega.
+  rewrite Znth_map', Znth_rev; [|omega].
+  rewrite Hlenl1, combine_app, map_app, sepcon_app.
+  instantiate (1 := (Tsh, Tsh)).
+  rewrite Z2Nat.inj_add, upto_app; try omega.
+  change (upto (Z.to_nat 1)) with [0]; simpl.
+  rewrite Z2Nat.id, map_app, sepcon_app, Z.add_0_r; [|omega].
+  simpl; replace (3 - Zlength vals - 1) with (2 - Zlength vals) by (clear; abstract omega).
+  rewrite app_Znth2, Zminus_diag; [simpl | clear; omega].
+  rewrite <- lock_struct_array; unfold fold_right at 3 4 5; cancel.
+  apply sepcon_derives; [apply derives_refl|].
+  apply derives_refl'; f_equal.
+  rewrite Zlength_correct, Nat2Z.id; apply map_ext_in; intros.
+  rewrite app_Znth1; auto.
+  rewrite In_upto in H; rewrite Zlength_correct; clear - H; omega.
+  { apply Nat2Z.inj; rewrite <- !Zlength_correct.
+    rewrite Zlength_sublist; try rewrite Zlength_map, Zlength_rev; abstract omega. }
+Qed.
+
+Transparent upto.
 
 Lemma body_main: semax_body Vprog Gprog f_main main_spec.
 Proof.
@@ -760,6 +548,7 @@ Proof.
             fold_right sepcon emp (map (fun x => lock_inv Tsh (snd x) (f_lock x)) (combine (upto (Z.to_nat i)) flocks)) *
             fold_right sepcon emp (map (fun x => malloc_token Tsh (sizeof tlock) x) flocks))))).
   { Exists ([] : list val); entailer!.
+    apply sepcon_derives; [simple apply derives_refl|].
     unfold data_at_, field_at_; simpl; cancel. }
   { forward_call (sizeof tlock).
     { admit. (* lock size broken *) }
@@ -772,7 +561,8 @@ Proof.
     forward_call (l, Tsh, f_lock (i, l)).
     { apply prop_right; rewrite sem_cast_neutral_ptr; rewrite sem_cast_neutral_ptr; auto. }
     { rewrite memory_block_data_at_; auto; simpl; cancel. }
-    Exists (flocks ++ [l]); rewrite Zlength_app, Zlength_cons, Zlength_nil, Forall_app; entailer!.
+    Exists (flocks ++ [l]); rewrite Zlength_app, Zlength_cons, Zlength_nil; entailer!.
+    { rewrite Forall_app; split; auto. }
     replace (Z.to_nat (3 - Zlength flocks)) with (S (Z.to_nat (3 - (Zlength flocks + 1)))); simpl.
     rewrite upd_Znth_app2, Zminus_diag, upd_Znth0, sublist_1_cons, sublist_same; auto; try rewrite Zlength_cons;
       try solve [rewrite !Zlength_correct; omega].
@@ -783,12 +573,13 @@ Proof.
     { exists 2; auto. } }
   Intros flocks.
   rewrite Zminus_diag, app_nil_r, <- seq_assoc.
+  erewrite add_andp with (P := data_at_ _ _ _); [|apply data_at__local_facts]; Intros.
   forward_for_simple_bound 3 (EX i : Z,
     PROP ()
     LOCAL (temp _t'1 q; gvar _results results; gvar _thread_locks locks; gvar _q0 q0)
     SEP (lqueue (fst (Znth (3 - i) lshs1 (Tsh, Tsh))) tint (is_int I32 Signed) q lock sh1 sh2 [];
          data_at_ Ews (tarray (tarray tint 3) (3 - i))
-           (offset_val (nested_field_offset (tarray tint 3) [ArraySubsc i]) results);
+           (offset_val (nested_field_offset (tarray (tarray tint 3) 3) [ArraySubsc i]) results);
          field_at (fst (Znth (3 - i) gshs1 (Ews, Ews))) (tptr tqueue_t) [] q q0;
          data_at (fst (Znth (3 - i) gshs1 (Ews, Ews))) (tarray (tptr (Tstruct _lock_t noattr)) 3) flocks locks;
          fold_right sepcon emp (map (fun x => lock_inv sh1 (snd x) (f_lock x)) (sublist 0 i (combine (upto 3) flocks)));
@@ -797,140 +588,147 @@ Proof.
   { rewrite sublist_nil, sublist_same; auto; [|rewrite Zlength_combine, Zlength_upto, Z.min_l; simpl; omega].
     entailer!.
     rewrite !Znth_overflow; try omega; simpl; cancel. }
-  { semax_subcommand Vprog Gprog f_main.
-apply main_loop1; auto. }
-  simpl; Intros flocks.
-  rewrite <- seq_assoc.
+  { apply main_loop1; auto. }
+  rewrite Zminus_diag.
+  rewrite sublist_nil, sublist_same; auto; [|rewrite Zlength_combine, Zlength_upto, Z.min_l; simpl; omega].
   set (lsh' := fst (Znth 0 lshs1 (Tsh, Tsh))).
   set (gsh' := fst (Znth 0 gshs1 (Ews, Ews))).
+  assert (readable_share gsh').
+  { exploit (Hgshs1 0); [computable|].
+    subst gsh'; destruct (Znth 0 gshs1 (Ews, Ews)) eqn: Hg1; setoid_rewrite Hg1; intros (? & ?); auto. }
+  forward.
+  rewrite <- seq_assoc.
+  forward_for_simple_bound 9 (EX i : Z,
+    PROP ()
+    LOCAL (temp _q1 q; temp _t'1 q; gvar _results results; gvar _thread_locks locks; gvar _q0 q0)
+    SEP (EX ptrs : list val, !!(Zlength ptrs = i) && lqueue lsh' tint (is_int I32 Signed) q lock sh1 sh2
+          (map (fun x => QAdd (fst x) (vint (snd x))) (combine ptrs (upto (Z.to_nat i))));
+         field_at gsh' (tptr tqueue_t) [] q q0;
+         data_at gsh' (tarray (tptr (Tstruct _lock_t noattr)) 3) flocks locks;
+         fold_right sepcon emp (map (fun x => lock_inv sh1 (snd x) (f_lock x)) (combine (upto 3) flocks));
+         fold_right sepcon emp (map (fun x => malloc_token Tsh (sizeof tlock) x) flocks))).
+  { Exists ([] : list val); entailer!.
+    unfold data_at_, field_at_, field_at, at_offset.
+    rewrite data_at_rec_eq; unfold unfold_reptype, default_val; simpl.
+    rewrite array_pred_len_0; [entailer! | auto]. }
+  { forward_call (sizeof tint).
+    { simpl; cancel. }
+    { simpl; computable. }
+    Intros d ptrs.
+    rewrite malloc_compat; auto; Intros.
+    rewrite memory_block_data_at_; auto.
+    forward.
+    forward_call (lsh', existT (fun t => ((reptype t -> Prop) * hist (reptype t) * reptype t)%type) tint
+      (is_int I32 Signed, map (fun x => QAdd (fst x) (vint (snd x))) (combine ptrs (upto (Z.to_nat i))), vint i),
+      q, lock, d, sh1, sh2).
+    { simpl; cancel. }
+    { exploit (Hlshs1 0); [computable|].
+      subst lsh'; destruct (Znth 0 lshs1 (Tsh, Tsh)) eqn: Hg1; intros (? & ?); auto. }
+    Exists (ptrs ++ [d]); rewrite Zlength_app, Zlength_cons, Zlength_nil; entailer!.
+    unfold fold_right; rewrite Z2Nat.inj_add, upto_app, combine_app, map_app; try omega; simpl.
+    rewrite Z2Nat.id, Z.add_0_r, Zlength_correct, Nat2Z.id; [cancel | omega].
+    simple apply derives_refl.
+    { rewrite upto_length, Zlength_correct, Nat2Z.id; auto. }
+    { exists 2; auto. } }
+  Intros ptrs.
+  rewrite <- seq_assoc.
   forward_for_simple_bound 3 (EX i : Z,
     PROP ()
-    LOCAL (temp _t'1 q; lvar _tid (tarray tint 3) lvar0; gvar _results results; gvar _thread_locks locks;
-           gvar _q0 q0)
-    SEP (EX ptrs : list val, !!(Zlength ptrs = i) && lqueue lsh' tint (is_int I32 Signed) q lock sh1 sh2
-          (map (fun x => QAdd (fst x) (vint (snd x))) (combine ptrs (upto i)));
-         field_at gsh' (tptr tqueue_t) [] q q0;
-         data_at sh1' (tarray (tptr (Tstruct _lock_t noattr)) 3) flocks locks;
-         fold_right sepcon emp (map (fun x => lock_inv sh1 (snd x) (f_lock x)) (combine (upto 3) flocks))))).
-  { go_lower; simpl.
-    Exists ([] : list val); entailer!.
-    do 2 (rewrite Znth_overflow with (i := 3); [simpl; cancel | abstract omega]). }
-  { semax_subcommand Vprog Gprog f_main.
-apply main_loop2; auto. }
-
-  simpl; Intro glocks; Intros.
-  rewrite <- seq_assoc.
-  forward_for_simple_bound 6 (EX i : Z,
-    PROP (Forall isptr flocks; Forall isptr glocks)
-    LOCAL (temp _t'1 p; lvar _thread_locks (tarray (tptr (Tstruct _lock_t noattr)) 6) lvar0; gvar _q0 q0)
-    SEP (ghost_factory; data_at (fst (Znth 0 gshs2 (gsh', gsh'))) (tptr tqueue_t) p q0;
-         fold_right sepcon emp (firstn (Z.to_nat i) (map (fun sh => data_at sh (tptr tqueue_t) p q0) (map snd (rev gshs1 ++ rev gshs2))));
-         lqueue (fst (Znth 0 lshs2 (lsh', lsh'))) gsh2 p ghosts lock;
-         fold_right sepcon emp (firstn (Z.to_nat i) (map (fun sh => lqueue sh gsh2 p ghosts lock) (map snd (rev lshs1 ++ rev lshs2))));
-         EX ns : list Z, (!!(Zlength ns = Zlength ghosts) &&
-           fold_right sepcon emp (firstn (Z.to_nat i - 3) (map (fun x => ghost gsh1 tint (vint (fst x)) (snd x)) (combine ns ghosts))));
-         fold_right sepcon emp (skipn (Z.to_nat i) (map Interp (map f_lock (combine (upto 3) flocks))));
-         fold_right sepcon emp (skipn (Z.to_nat i - 3) (map Interp (map g_lock (combine (upto 3) glocks))));
-         data_at Tsh (tarray (tptr (Tstruct _lock_t noattr)) 6) (flocks ++ glocks) lvar0)).
-  { go_lower; apply andp_right; [|rewrite app_nil_r; Exists [0; 0; 0]; entailer!].
-    Intros.
-    do 3 (destruct flocks; [Omega0|]).
-    do 3 (destruct glocks; [Omega0|]).
-    repeat rewrite Zlength_cons in *; unfold Z.succ in *.
-    assert (flocks = []) by (apply Zlength_nil_inv; abstract omega).
-    assert (glocks = []) by (apply Zlength_nil_inv; abstract omega).
-    Transparent upto.
-    subst; simpl.
-    rewrite (lock_inv_isptr _ v), (lock_inv_isptr _ v0), (lock_inv_isptr _ v1), (lock_inv_isptr _ v2),
-      (lock_inv_isptr _ v3), (lock_inv_isptr _ v4).
-    rewrite !sepcon_assoc, !sepcon_andp_prop', !sepcon_andp_prop.
-    repeat (apply derives_extract_prop; intro).
-    apply prop_right; repeat split; auto. }
-  { semax_subcommand Vprog Gprog f_main.
-apply main_loop3; auto. }
-  Intro ns; Intros.
-  rewrite !Zfirstn_same; try (rewrite !Zlength_map, Zlength_app, !Zlength_rev; abstract omega).
-  rewrite !map_app, !sepcon_app, !map_rev, !sepcon_rev.
-  rewrite sepcon_comm; gather_SEP 1 2.
-  rewrite <- sepcon_assoc, data_at_shares_join; [|rewrite Hglen2; auto].
-  subst gsh'; rewrite data_at_shares_join; [|rewrite Hglen1; auto].
-  rewrite sepcon_comm; gather_SEP 2 3.
-  rewrite <- sepcon_assoc, lqueue_shares_join; [|rewrite Hlenl2; auto].
-  subst lsh'; rewrite lqueue_shares_join; [|rewrite Hlenl1; auto].
+    LOCAL (temp _q1 q; temp _t'1 q; gvar _results results; gvar _thread_locks locks; gvar _q0 q0)
+    SEP (field_at gsh' (tptr tqueue_t) [] q q0;
+         fold_right sepcon emp (sublist 0 i (map (fun sh => data_at sh (tptr tqueue_t) q q0) (map snd (rev gshs1))));
+         data_at gsh' (tarray (tptr (Tstruct _lock_t noattr)) 3) flocks locks;
+         fold_right sepcon emp (sublist 0 i (map (fun sh => data_at_ sh (tarray (tptr (Tstruct _lock_t noattr)) 3) locks) (map snd (rev gshs1))));
+         fold_right sepcon emp (sublist i 3 (map (fun x => lock_inv sh1 (snd x) (f_lock x)) (combine (upto 3) flocks)));
+         fold_right sepcon emp (sublist i 3 (map (fun x => malloc_token Tsh (sizeof tlock) x) flocks));
+         lqueue lsh' tint (is_int I32 Signed) q lock sh1 sh2
+          (map (fun x => QAdd (fst x) (vint (snd x))) (combine ptrs (upto (Z.to_nat 9))));
+         EX vals : list (list (val * int)), !!(Zlength vals = i /\ Forall (fun l => Zlength l = 3) vals) &&
+         (fold_right sepcon emp (map (fun x => let '(sh, vals) := x in
+            lqueue sh tint (is_int I32 Signed) q lock sh1 sh2
+              (map (fun x => let '(p, i) := x in QRem p (Vint i)) vals))
+            (combine (sublist 0 i (map snd (rev lshs1))) vals)) *
+          fold_right sepcon emp (map (fun x => field_at Ews (tarray (tarray tint 3) 3) [ArraySubsc x]
+            (map Vint (map snd (Znth x vals []))) results) (upto (Z.to_nat i)))))).
+  { rewrite !sublist_nil; rewrite !sublist_same; auto;
+      try rewrite Zlength_map; try rewrite Zlength_combine, Zlength_upto, Z.min_l; auto; [|simpl; omega].
+    Exists ([] : list (list (val * int))); entailer!. }
+  { simple apply main_loop2 with (q2 := q)(locks0 := locks)(q1 := q0)(gshs2 := gshs1)
+      (lshs2 := lshs1)(sh3 := sh1)(sh4 := sh2)(lock0 := lock); auto. }
+  Intros vals.
+  rewrite !sublist_nil, !sublist_same; auto; rewrite ?Zlength_map, ?Zlength_rev; auto.
+  rewrite !map_rev, !sepcon_rev.
+  change (field_at gsh' (tptr tqueue_t) [] q q0) with (data_at gsh' (tptr tqueue_t) q q0).
+  gather_SEP 0 1; subst gsh'; rewrite data_at_shares_join; [|rewrite Hglen1; auto].
+  gather_SEP 1 2; replace_SEP 0 (...) by (go_lowerx; apply data_at__shares_join; rewrite Hglen1; auto).
+  gather_SEP 4 5; replace_SEP 0 (EX h' : hist (reptype tint),
+    !!(interleave (map (fun x => QAdd (fst x) (vint (snd x))) (combine ptrs (upto (Z.to_nat 9))) ::
+                   map (fun vals => map (fun x => let '(p, i) := x in QRem p (Vint i)) vals) (rev vals)) h') &&
+    lqueue Tsh tint (is_int I32 Signed) q lock sh1 sh2 h').
+  { assert (length lshs1 = length (map (fun vals => map (fun x => let '(p, i) := x in
+      QRem p (Vint i)) vals) (rev vals))).
+    { rewrite !map_length, rev_length; rewrite Zlength_correct in *; abstract omega. }
+    go_lowerx; eapply derives_trans; [|apply lqueue_shares_join; [eauto | rewrite Hlenl1; eauto]].
+    subst lsh'; cancel.
+    rewrite combine_map_snd, map_map.
+    rewrite <- sepcon_rev, <- map_rev, rev_combine, rev_involutive.
+    erewrite map_ext; [apply derives_refl|].
+    destruct a; auto.
+    { rewrite rev_length, map_length, rev_length in *; auto. } }
+  Intros h'.
+  repeat (destruct ptrs; [rewrite Zlength_nil in *; discriminate | rewrite Zlength_cons in *]).
+  destruct ptrs; [|rewrite Zlength_cons, Zlength_correct in *; omega].
+  repeat (destruct vals; [rewrite Zlength_nil in *; discriminate | rewrite Zlength_cons in *]).
+  destruct vals; [|rewrite Zlength_cons, Zlength_correct in *; omega].
+  repeat match goal with H : Forall _ (_ :: _) |- _ => inv H end.
+  repeat (destruct l as [|(?, ?)]; [rewrite Zlength_nil in *; discriminate | rewrite Zlength_cons in *]).
+  destruct l; [|rewrite Zlength_cons, Zlength_correct in *; omega].
+  repeat (destruct l0 as [|(?, ?)]; [rewrite Zlength_nil in *; discriminate | rewrite Zlength_cons in *]).
+  destruct l0; [|rewrite Zlength_cons, Zlength_correct in *; omega].
+  repeat (destruct l1 as [|(?, ?)]; [rewrite Zlength_nil in *; discriminate | rewrite Zlength_cons in *]).
+  destruct l1; [|rewrite Zlength_cons, Zlength_correct in *; omega].
+  simpl in *.
+  rewrite lqueue_feasible; Intros.
+  assert (consistent h' [] [] /\ interleave [[Vint i; Vint i0; Vint i1]; [Vint i2; Vint i3; Vint i4];
+    [Vint i5; Vint i6; Vint i7]] [vint 0; vint 1; vint 2; vint 3; vint 4; vint 5; vint 6; vint 7; vint 8])
+    as (? & ?).
+  { match goal with H : feasible h' |- _ => destruct H as (b & Hcon) end.
+    exploit (@add_first (reptype tint)); try eassumption.
+    clear - Hcon.
+    intros (h1 & h2 & Hadds & Hrems & Hcon'); simpl in *.
+    rewrite interleave_remove_nil in Hrems.
+    repeat setoid_rewrite interleave_remove_nil' with (ls1 := [_]) in Hadds.
+    rewrite app_nil_r, interleave_single in Hadds.
+    exploit (consistent_adds h1); subst; auto.
+    intros (l & Hl & Hh1).
+    repeat (destruct l as [|(?, ?)]; [discriminate|]); destruct l; [|discriminate].
+    simpl in Hl; inv Hl.
+    rewrite Hh1 in Hcon'.
+    exploit (consistent_rems h2).
+    { rewrite forallb_forall; intros ? Hin.
+      rewrite interleave_In in Hin; [|eassumption].
+      simpl in Hin; destruct Hin as (? & [? | [? | [? | ?]]] & Hin); try contradiction; subst;
+        destruct Hin as [? | [? | [? | ?]]]; try contradiction; subst; auto. }
+    { eassumption. }
+    intros (? & ? & ?); subst.
+    pose proof (Zlength_interleave _ _ Hrems) as Hlen.
+    rewrite Zlength_map in Hlen; simpl in Hlen.
+    assert (Zlength (x ++ b) = 9) by (rewrite <- H; Omega0).
+    destruct b; [|rewrite Zlength_app, Zlength_cons in *; rewrite !Zlength_correct in *; omega].
+    split; auto.
+    rewrite app_nil_r in *; subst; simpl in *.
+    eapply interleave_combine.
+    { instantiate (1 := [[_; _; _]; [_; _; _]; [_; _; _]]).
+      repeat (constructor; [simpl; reflexivity|]); auto. }
+    { instantiate (1 := [_; _; _; _; _; _; _; _; _]); simpl; auto. }
+    apply (interleave_map_inj (fun x => let '(p, v) := x in @QRem (reptype tint) p v)); simpl.
+    { intros (?, ?) (?, ?) Heq; inv Heq; auto. }
+    setoid_rewrite interleave_reorder with (ls1 := [_]) in Hrems.
+    setoid_rewrite interleave_reorder with (ls1 := [_; _]) in Hrems.
+    apply Hrems. }
+  forward_call (existT (fun t => ((reptype t -> Prop) * hist (reptype t))%type) tint (is_int I32 Signed, h'),
+                q, lock, sh1, sh2).
   forward.
-  forward_call (gsh1, gsh2, p, ghosts, ns, lock).
-  { replace (Z.to_nat 6 - 3)%nat with (Z.to_nat 3)%nat by Omega0.
-    rewrite Zfirstn_same; simpl.
-    unfold fold_right at 3; cancel.
-    { rewrite Zlength_map, Zlength_combine, Z.min_l; try abstract omega.
-      subst ghosts; rewrite !Zlength_cons, Zlength_nil in *; abstract omega. } }
-  forward.
-  Exists lvar0; entailer!.
-Qed.
-
-(*
-(* linking *)
-Require Import progs.verif_conc_queue.
-
-Lemma Gprog_sub : incl verif_conc_queue.Gprog Gprog.
-Proof.
-  unfold verif_conc_queue.Gprog, Gprog.
-  repeat apply incl_same_head.
-  do 3 apply incl_tl; repeat apply incl_same_head; auto.
-Qed.
-
-Definition extlink := ext_link_prog prog.
-
-Definition Espec := add_funspecs (Concurrent_Espec unit _ extlink) extlink Gprog.
-Existing Instance Espec.
-
-(* Use semax_func_mono here. *)
-Lemma all_funcs_correct:
-  semax_func Vprog Gprog (prog_funct prog) Gprog.
-Proof.
-unfold Gprog, prog, prog_funct; simpl.
-repeat (apply semax_func_cons_ext_vacuous; [reflexivity | reflexivity |]).
-eapply semax_func_cons_ext; try reflexivity.
-{ intros; entailer!. }
-{ admit. }
-eapply semax_func_cons_ext; try reflexivity.
-{ admit. }
-{ admit. }
-semax_func_cons_ext.
-semax_func_cons_ext.
-semax_func_cons_ext.
-semax_func_cons_ext.
-semax_func_cons_ext.
-semax_func_cons_ext.
-semax_func_cons_ext.
-semax_func_cons_ext.
-semax_func_cons_ext.
-semax_func_cons_ext.
-semax_func_cons_ext.
-semax_func_cons body_get_request.
-semax_func_cons body_process_request.
-semax_func_cons body_q_new.
-semax_func_cons body_q_del.
-semax_func_cons body_q_add.
-semax_func_cons body_q_remove.
-semax_func_cons body_f.
-(* XX For some reason, precondition_closed can't prove that all the gvars
-   aren't local variables. *)
-apply semax_func_cons; 
- [ reflexivity 
- | repeat apply Forall_cons; try apply Forall_nil; auto; computable
- | unfold var_sizes_ok; repeat constructor; simpl; computable | reflexivity
- | | apply body_g | ].
-{ precondition_closed.
-  apply closed_wrtl_PROPx, closed_wrtl_LOCALx, closed_wrtl_SEPx.
-  repeat constructor; apply closed_wrtl_gvar; unfold is_a_local; simpl;
-    intros [? | ?]; try contradiction; discriminate. }
-(* Here it's just missing an auto. *)
-apply semax_func_cons; 
- [ reflexivity 
- | repeat apply Forall_cons; try apply Forall_nil; (*here*)auto; computable
- | unfold var_sizes_ok; repeat constructor; simpl; computable | reflexivity
- | precondition_closed | apply body_main | ].
-apply semax_func_nil.
 Admitted.
-*)
+
+(* For linking, see verif_queue_ex_linking. *)
